theories/OGS/Machine.v
@@ -1,0 +1,48 @@
+From OGS Require Import Prelude.
+From OGS.Utils Require Import Ctx Rel.
+From OGS.Game Require Import HalfGame Event.
+From OGS.OGS Require Import Subst Obs.
+From OGS.ITree Require Import ITree Eq Delay Structure Properties Guarded.
+
+Section withFam.
+  Context {bT : baseT}.
+  Context {bV : baseV}.
+  Context {bC : baseC}.
+  Context {sV : subst_monoid bV}.
+  Context {sC : subst_module bV bC}.
+  Context {oS : observation_structure}.
+
+  Class machine : Type := {
+      eval {Γ} : conf Γ -> delay (nf' Γ) ;
+      app {Γ x} (v : val Γ x) (m : obs x) (r : dom m ⇒ᵥ Γ) : conf Γ ;
+    }.
+
+  Context {M : machine}.
+
+  Definition eval_to_obs {Γ} (t : conf Γ) : delay (obs∙ Γ) :=
+    fmap_delay (obs'_of_nf' Γ) (eval t) .
+
+  Variant head_inst_nostep (u : { x : typ & obs x }) : { x : typ & obs x } -> Prop :=
+  | HeadInst {Γ y} (v : val Γ y) (m : obs y) (e : dom m ⇒ᵥ Γ) (p : is_var v -> False) (i : Γ ∋ projT1 u)
+             : eval_to_obs (app v m e) ≊ ret_delay (projT1 u ,' (i , projT2 u)) ->
+               head_inst_nostep u (y ,' m) .
+
+  Class machine_laws : Prop := {
+    app_proper {Γ x v m} :: Proper (ass_eq (dom m) Γ ==> eq) (@app _ Γ x v m) ;
+
+    app_sub {Γ1 Γ2 x} (e : Γ1 ⇒ᵥ Γ2) (v : val Γ1 x) (m : obs x) (r : dom m ⇒ᵥ Γ1)
+      : e ⊛ₜ app v m r = app (e ⊛ᵥ v) m (e ⊛ r) ;
+
+    eval_sub {Γ Δ} (c : conf Γ) (e : Γ ⇒ᵥ Δ)
+      : eval (e ⊛ₜ c)
+      ≋ bind_delay' (eval c) (fun u => eval (app (e _ (nf'_var u)) (nf'_obs u) (e ⊛ nf'_val u))) ;
+
+    eval_nf_ret {Γ} (u : nf' Γ) :
+      eval (app (v_var _ (nf'_var u)) (nf'_obs u) (nf'_val u))
+      ≋ ret_delay u ;
+
+    eval_app_not_var : well_founded head_inst_nostep ;
+  } .
+
+
+End withFam.
