theories/OGS/Obs.v
@@ -1,0 +1,95 @@
+From OGS Require Import Prelude.
+From OGS.Utils Require Import Ctx Rel.
+From OGS.Game Require Import HalfGame Event.
+From OGS.OGS Require Import Subst.
+From OGS.ITree Require Import Delay Eq.
+
+Open Scope ctx_scope.
+
+Section withFam.
+  Context {bT : baseT}.
+
+(*|
+Observation Structure (§ 5.4)
+==============================
+
+The messages that player and opponent exchange in the OGS
+arise from splitting normal forms into the head variable
+on which it is stuck, an observation, and an assignment.
+
+An **observation structure** axiomatizes the observations
+of the language:
+- a Type [typ] of types (assumed globally in Section 5),
+- a type-indexed set [obs] of observations,
+- a map [dom] mapping observations to values filling their copattern
+
+|*)
+  Class observation_structure : Type := {
+      obs : typ -> Type ;
+      dom : forall t, obs t -> ctx typ ;
+    }.
+  Arguments dom {_} [_].
+
+  Context {O : observation_structure}.
+
+(*|
+Given an observation structure, we define the family of pointed observations
+(Definition 5.15) packaging them into a type, and an observation at
+this type.
+|*)
+  Notation context := (ctx typ).
+  Definition obs' (Γ : context) : Type := { t : typ & Γ ∋ t * obs t }%type.
+  Notation "obs∙" := obs'.
+
+  Definition obs'_ty {Γ} (o : obs∙ Γ) : typ := projT1 o.
+  Notation "ty∙ o" := (obs'_ty o) (at level 10).
+  Definition obs'_var {Γ} (o : obs∙ Γ) : Γ ∋ ty∙ o := fst (projT2 o).
+  Definition obs'_obs {Γ} (o : obs∙ Γ) : obs (ty∙ o) := snd (projT2 o).
+  Definition obs'_dom {Γ} (o : obs∙ Γ) : context := dom (obs'_obs o).
+  Notation "dom∙ o" := (obs'_dom o) (at level 10).
+
+(*|
+Given an observation structure and a sorted family of values,
+we can define normal forms as a pair of a pointed observation and an
+assignment for its domain.
+The following definition is equivalent, but with a slightly different packaging.
+|*)
+  Context {bV : baseV}.
+  Context {sV : subst_monoid bV}.
+
+  Definition nf  (Γ : context) (t : typ) : Type := { m : obs t & dom m ⇒ᵥ Γ }.
+  Definition nf' (Γ : context) : Type := { t : typ & Γ ∋ t * nf Γ t }%type.
+  Notation "nf∙" := nf'.
+
+  Definition nf'_ty {Γ} : nf∙ Γ -> typ := @projT1 _ _.
+  Definition nf'_var {Γ} (u : nf∙ Γ) : Γ ∋ (nf'_ty u) := fst (projT2 u).
+  Definition nf'_nf {Γ} (u : nf∙ Γ) : nf Γ (nf'_ty u) := snd (projT2 u).
+  Definition nf'_obs {Γ} (u : nf∙ Γ) : obs (nf'_ty u) := projT1 (snd (projT2 u)).
+  Definition nf'_val {Γ} (u : nf∙ Γ) : dom (nf'_obs u) ⇒ᵥ Γ := projT2 (snd (projT2 u)).
+
+  Definition nf_eq {Γ t} : relation (nf Γ t) :=
+    fun a b => exists H : projT1 a = projT1 b,
+        rew H in projT2 a ≡ₐ projT2 b.
+
+  Definition nf'_eq {Γ} : relation (nf∙ Γ) :=
+    fun a b => exists H : nf'_ty a = nf'_ty b,
+        (rew H in nf'_var a = nf'_var b) /\ (nf_eq (rew H in nf'_nf a) (nf'_nf b)).
+
+  Definition comp_eq {Γ} : relation (delay (nf∙ Γ)) :=
+    it_eq (fun _ : T1 => nf'_eq) (i := T1_0).
+  Notation "u ≋ v" := (comp_eq u v) (at level 40).
+
+  Definition obs'_of_nf' : nf∙ ⇒ᵢ obs∙ :=
+    fun Γ u => (nf'_ty u ,' (nf'_var u , nf'_obs u)).
+
+  Definition nf'_of_obs' {Γ} (o : obs∙ Γ) : nf∙ (Γ +▶ dom∙ o) :=
+    (obs'_ty o ,' (r_concat_l _ (obs'_var o) , (obs'_obs o ,' v_var ⊛ᵣ r_concat_r))).
+
+End withFam.
+
+Arguments dom {_ _} [_].
+#[global] Notation "obs∙ Γ" := (obs' Γ) (at level 10).
+#[global] Notation "ty∙ o" := (obs'_ty o) (at level 10).
+#[global] Notation "dom∙ o" := (obs'_dom o) (at level 10).
+#[global] Notation "nf∙ Γ" := (nf' Γ) (at level 10).
+#[global] Notation "u ≋ v" := (comp_eq u v) (at level 40).
